Prove type soundness for the updated FFI

semantics/proofs/typeSoundInvariantsScript.sml
@@ -75,87 +75,87 @@ val add_tenvE_def = Define `
   (add_tenvE (Bind_name x tvs t tenvE) tenvV = nsBind x (tvs,t) (add_tenvE tenvE tenvV))`;
 
 val (type_v_rules, type_v_cases, type_v_ind) = Hol_reln `
-  (!tvs ctMap tenvS n.
-    type_v tvs ctMap tenvS (Litv (IntLit n)) Tint) ∧
-  (!tvs ctMap tenvS c.
-    type_v tvs ctMap tenvS (Litv (Char c)) Tchar) ∧
-  (!tvs ctMap tenvS s.
-    type_v tvs ctMap tenvS (Litv (StrLit s)) Tstring) ∧
-  (!tvs ctMap tenvS w.
-    type_v tvs ctMap tenvS (Litv (Word8 w)) Tword8) ∧
-  (!tvs ctMap tenvS w.
-    type_v tvs ctMap tenvS (Litv (Word64 w)) Tword64) ∧
-  (!tvs ctMap tenvS vs tvs' stamp ts' ts ti.
+  (!signs tvs ctMap tenvS n.
+    type_v signs tvs ctMap tenvS (Litv (IntLit n)) Tint) ∧
+  (!signs tvs ctMap tenvS c.
+    type_v signs tvs ctMap tenvS (Litv (Char c)) Tchar) ∧
+  (!signs tvs ctMap tenvS s.
+    type_v signs tvs ctMap tenvS (Litv (StrLit s)) Tstring) ∧
+  (!signs tvs ctMap tenvS w.
+    type_v signs tvs ctMap tenvS (Litv (Word8 w)) Tword8) ∧
+  (!signs tvs ctMap tenvS w.
+    type_v signs tvs ctMap tenvS (Litv (Word64 w)) Tword64) ∧
+  (!signs tvs ctMap tenvS vs tvs' stamp ts' ts ti.
     EVERY (check_freevars tvs []) ts' ∧
     LENGTH tvs' = LENGTH ts' ∧
-    LIST_REL (type_v tvs ctMap tenvS)
+    LIST_REL (type_v signs tvs ctMap tenvS)
       vs (MAP (type_subst (FUPDATE_LIST FEMPTY (REVERSE (ZIP (tvs', ts'))))) ts) ∧
     FLOOKUP ctMap stamp = SOME (tvs',ts,ti)
     ⇒
-    type_v tvs ctMap tenvS (Conv (SOME stamp) vs) (Tapp ts' ti)) ∧
-  (!tvs ctMap tenvS vs ts.
-    LIST_REL (type_v tvs ctMap tenvS) vs ts
+    type_v signs tvs ctMap tenvS (Conv (SOME stamp) vs) (Tapp ts' ti)) ∧
+  (!signs tvs ctMap tenvS vs ts.
+    LIST_REL (type_v signs tvs ctMap tenvS) vs ts
     ⇒
-    type_v tvs ctMap tenvS (Conv NONE vs) (Ttup ts)) ∧
+    type_v signs tvs ctMap tenvS (Conv NONE vs) (Ttup ts)) ∧
   (!signs tvs ctMap tenvS env tenv tenvE n e t1 t2.
     tenv_ok tenv ∧
     tenv_val_exp_ok tenvE ∧
     num_tvs tenvE = 0 ∧
     nsAll2 (type_ctor ctMap) env.c tenv.c ∧
-    nsAll2 (\i v (tvs,t). type_v tvs ctMap tenvS v t) env.v (add_tenvE tenvE tenv.v) ∧
+    nsAll2 (\i v (tvs,t). type_v signs tvs ctMap tenvS v t) env.v (add_tenvE tenvE tenv.v) ∧
     check_freevars tvs [] t1 ∧
     type_e signs tenv (Bind_name n 0 t1 (bind_tvar tvs tenvE)) e t2
     ⇒
-    type_v tvs ctMap tenvS (Closure env n e) (Tfn t1 t2)) ∧
+    type_v signs tvs ctMap tenvS (Closure env n e) (Tfn t1 t2)) ∧
   (!signs tvs ctMap tenvS env funs n t tenv tenvE bindings.
     tenv_ok tenv ∧
     tenv_val_exp_ok tenvE ∧
     num_tvs tenvE = 0 ∧
     nsAll2 (type_ctor ctMap) env.c tenv.c ∧
-    nsAll2 (\i v (tvs,t). type_v tvs ctMap tenvS v t) env.v (add_tenvE tenvE tenv.v) ∧
+    nsAll2 (\i v (tvs,t). type_v signs tvs ctMap tenvS v t) env.v (add_tenvE tenvE tenv.v) ∧
     type_funs signs tenv (bind_var_list 0 bindings (bind_tvar tvs tenvE)) funs bindings ∧
     ALOOKUP bindings n = SOME t ∧
     ALL_DISTINCT (MAP FST funs) ∧
     MEM n (MAP FST funs)
     ⇒
-    type_v tvs ctMap tenvS (Recclosure env funs n) t) ∧
-  (!tvs ctMap tenvS n t.
+    type_v signs tvs ctMap tenvS (Recclosure env funs n) t) ∧
+  (!signs tvs ctMap tenvS n t.
     check_freevars 0 [] t ∧
     FLOOKUP tenvS n = SOME (Ref_t t)
     ⇒
-    type_v tvs ctMap tenvS (Loc n) (Tref t)) ∧
-  (!tvs ctMap tenvS n.
+    type_v signs tvs ctMap tenvS (Loc n) (Tref t)) ∧
+  (!signs tvs ctMap tenvS n.
     FLOOKUP tenvS n = SOME W8array_t
     ⇒
-    type_v tvs ctMap tenvS (Loc n) Tword8array) ∧
-  (!tvs ctMap tenvS n t.
+    type_v signs tvs ctMap tenvS (Loc n) Tword8array) ∧
+  (!signs tvs ctMap tenvS n t.
     check_freevars 0 [] t ∧
     FLOOKUP tenvS n = SOME (Varray_t t)
     ⇒
-    type_v tvs ctMap tenvS (Loc n) (Tarray t)) ∧
-  (!tvs ctMap tenvS vs t.
+    type_v signs tvs ctMap tenvS (Loc n) (Tarray t)) ∧
+  (!signs tvs ctMap tenvS vs t.
     check_freevars 0 [] t ∧
-    EVERY (\v. type_v tvs ctMap tenvS v t) vs
+    EVERY (\v. type_v signs tvs ctMap tenvS v t) vs
     ⇒
-    type_v tvs ctMap tenvS (Vectorv vs) (Tvector t))`;
+    type_v signs tvs ctMap tenvS (Vectorv vs) (Tvector t))`;
 
 val type_sv_def = Define `
-  (type_sv ctMap tenvS (Refv v) (Ref_t t) ⇔ type_v 0 ctMap tenvS v t) ∧
-  (type_sv ctMap tenvS (W8array v) W8array_t ⇔ T) ∧
-  (type_sv ctMap tenvS (Varray vs) (Varray_t t) ⇔
-    EVERY (\v. type_v 0 ctMap tenvS v t) vs) ∧
-  (type_sv _ _ _ _ ⇔ F)`;
+  (type_sv signs ctMap tenvS (Refv v) (Ref_t t) ⇔ type_v signs 0 ctMap tenvS v t) ∧
+  (type_sv signs ctMap tenvS (W8array v) W8array_t ⇔ T) ∧
+  (type_sv signs ctMap tenvS (Varray vs) (Varray_t t) ⇔
+    EVERY (\v. type_v signs 0 ctMap tenvS v t) vs) ∧
+  (type_sv _ _ _ _ _ ⇔ F)`;
 
 
 (* The type of the store *)
 val type_s_def = Define `
-  type_s ctMap envS tenvS ⇔
+  type_s signs ctMap envS tenvS ⇔
     (!l.
       ((?st. FLOOKUP tenvS l = SOME st) ⇔ (?v. store_lookup l envS = SOME v)) ∧
       (!st sv.
         FLOOKUP tenvS l = SOME st ∧ store_lookup l envS = SOME sv
         ⇒
-        type_sv ctMap tenvS sv st))`;
+        type_sv signs ctMap tenvS sv st))`;
 
 (* The global constructor type environment has the primitive exceptions in it *)
 val ctMap_has_exns_def = Define `
@@ -221,17 +221,17 @@ val decls_ok_def = Define `
   *)
 
 val type_all_env_def = Define `
-  type_all_env ctMap tenvS env tenv ⇔
+  type_all_env signs ctMap tenvS env tenv ⇔
     nsAll2 (type_ctor ctMap) (sem_env_c env) tenv.c ∧
-    nsAll2 (\i v (tvs,t). type_v tvs ctMap tenvS v t) (sem_env_v env) tenv.v`;
+    nsAll2 (\i v (tvs,t). type_v signs tvs ctMap tenvS v t) (sem_env_v env) tenv.v`;
 
 val type_sound_invariant_def = Define `
 type_sound_invariant st env ctMap tenvS type_idents tenv ⇔
   tenv_ok tenv ∧
   good_ctMap ctMap ∧
   consistent_ctMap st type_idents ctMap ∧
-  type_all_env ctMap tenvS env tenv ∧
-  type_s ctMap st.refs tenvS`;
+  type_all_env (st.ffi.signatures) ctMap tenvS env tenv ∧
+  type_s (st.ffi.signatures) ctMap st.refs tenvS`;
 
 
 val _ = export_theory();
